src/Oeuf.v
@@ -13,106 +13,30 @@ Require Import compcert.common.AST.
 Require compcert.backend.SelectLong.
 Require Import Linker.
 
+Definition transf_untyped_to_cminor (p : Untyped1.prog_type) :=
+        OK p
+    @@@ UntypedCompCombined.compile_cu
+    @@@ ElimFuncCompCombined.compile_cu
+    @@@ StackCompCombined.compile_cu
+    @@@ LocalsCompCombined.compile_cu
+    @@@ FlatCompCombined.compile_cu
 
-Definition transf_untyped_to_tagged (l : list Untyped1.expr * list Metadata.metadata) :=
-  OK l
- @@@ UntypedCompCombined.compile_cu
- @@@ TaggedComp.compile_cu ~~ "TaggedComp".
-
-Definition transf_untyped_to_tagged_numbered (l : list Untyped1.expr * list Metadata.metadata)  :=
-  OK l
-  @@@ transf_untyped_to_tagged
-  @@ TaggedNumberedComp.compile_cu.
-
-Definition transf_untyped_to_elim_func (l : list Untyped1.expr * list Metadata.metadata)  :=
-  OK l
-  @@@ transf_untyped_to_tagged_numbered
-  @@@ ElimFuncComp.compile_cu.
- 
-Definition transf_untyped_to_elim_func2 (l : list Untyped1.expr * list Metadata.metadata)  :=
-  OK l
-  @@@ transf_untyped_to_elim_func
-  @@@ ElimFuncComp2.compile_cu.
-
-Definition transf_untyped_to_elim_func3 (l : list Untyped1.expr * list Metadata.metadata)  :=
-  OK l
-  @@@ transf_untyped_to_elim_func2
-  @@@ ElimFuncComp3.compile_cu.
-
-Definition transf_untyped_to_switched (l : list Untyped1.expr * list Metadata.metadata)  :=
-  OK l
-  @@@ transf_untyped_to_elim_func3
-  @@@ SwitchedComp.compile_cu ~~ "SwitchedComp".
-
-Definition transf_untyped_to_self_close (l : list Untyped1.expr * list Metadata.metadata)  :=
-  OK l
-  @@@ transf_untyped_to_switched
-  @@ SelfCloseComp.compile_cu.
-
-Definition transf_untyped_to_value_flag (l : list Untyped1.expr * list Metadata.metadata)  :=
-  OK l
-  @@@ transf_untyped_to_self_close
-  @@ ValueFlagComp.compile_cu.
-
-Definition transf_untyped_to_stack (l : list Untyped1.expr * list Metadata.metadata)  :=
-  OK l
-  @@@ transf_untyped_to_value_flag
-  @@@ StackCompCombined.compile_cu.
-
-Definition transf_untyped_to_locals (l : list Untyped1.expr * list Metadata.metadata)  :=
-  OK l
-  @@@ transf_untyped_to_stack
-  @@@ LocalsCompCombined.compile_cu.
-
-Definition transf_untyped_to_flat (l : list Untyped1.expr * list Metadata.metadata)  :=
-  OK l
-  @@@ transf_untyped_to_locals
-  @@@ FlatCompCombined.compile_cu.
-
-Definition transf_untyped_to_fmajor (l : list Untyped1.expr * list Metadata.metadata)  :=
-  OK l
-  @@@ transf_untyped_to_flat
-  @@@ FmajorComp.compile_cu_intern ~~ "FmajorComp".
-
-Definition transf_untyped_to_fflatmajor (l : list Untyped1.expr * list Metadata.metadata)  :=
-  OK l
-  @@@ transf_untyped_to_fmajor
-  @@ Fmajortofflatmajor.transf_program.
-
-Definition transf_untyped_to_emajor (l : list Untyped1.expr * list Metadata.metadata)  :=
-  OK l
-  @@@ transf_untyped_to_fflatmajor
-  @@ Fflatmajortoemajor.transf_program.
-
-Definition transf_untyped_to_dmajor (l : list Untyped1.expr * list Metadata.metadata)  :=
-  OK l
-  @@@ transf_untyped_to_emajor
-  @@@ Emajortodmajor.transf_prog.
-
-Definition transf_untyped_to_dflatmajor (l : list Untyped1.expr * list Metadata.metadata)  :=
-  OK l
-  @@@ transf_untyped_to_dmajor
-  @@@ Dmajortodflatmajor.transf_prog.
-
-Definition transf_untyped_to_cmajor (l : list Untyped1.expr * list Metadata.metadata)  :=
-  OK l
-  @@@ transf_untyped_to_dflatmajor
-  @@@ Dflatmajortocmajor.transf_prog.
-
-
-Definition transf_untyped_to_cminor (l : list Untyped1.expr * list Metadata.metadata) : res Cminor.program :=
-  OK l
-  @@@ transf_untyped_to_cmajor
-  @@ Cmajortominor.transf_prog
-  @@ print print_Cminor.
-
+    @@@ FmajorComp.compile_cu_intern ~~ "FmajorComp"
+    @@  Fmajortofflatmajor.transf_program
+    @@  Fflatmajortoemajor.transf_program
+    @@@ Emajortodmajor.transf_prog
+    @@@ Dmajortodflatmajor.transf_prog
+    @@@ Dflatmajortocmajor.transf_prog
+    @@  Cmajortominor.transf_prog
+.
 
 Definition transf_oeuf_to_untyped1 (j : CompilationUnit.compilation_unit) : res Untyped1.prog_type :=
   OK (CompilationUnit.init_metadata j)
-  @@ UntypedComp1.compile_cu
- @@@ Metadata.check_length.
+ @@@ UntypedComp1.compile_cu ~~ "UntypedComp1"
+ @@@ Metadata.check_length ~~ "Metadata".
 
-Definition transf_oeuf_to_cminor (j : CompilationUnit.compilation_unit) : res Cminor.program :=
+Definition transf_oeuf_to_cminor (j : CompilationUnit.compilation_unit) :
+    res Cmajor.Cminor_program :=
      transf_oeuf_to_untyped1 j
  @@@ transf_untyped_to_cminor.
 
@@ -128,11 +52,11 @@ Definition transf_whole_program (oeuf_code : CompilationUnit.compilation_unit) (
   | OK oeuf_cm =>
     match transf_c_to_cminor shim_code with
     | OK shim_cm =>
-      match shim_link oeuf_cm shim_cm with
+      match shim_link (Cmajor.cm_ast oeuf_cm) shim_cm with
       | OK all_cm =>
         match transf_cminor_program all_cm with
         | OK all_asm =>
-          OK (oeuf_cm, shim_cm, all_cm, all_asm)
+          OK (Cmajor.cm_ast oeuf_cm, shim_cm, all_cm, all_asm)
         | Error m => Error m
         end
       | Error m => Error m
@@ -141,4 +65,4 @@ Definition transf_whole_program (oeuf_code : CompilationUnit.compilation_unit) (
     end
   | Error m => Error m
   end.
-                                    
+
